{
 "cells": [
  {
   "cell_type": "markdown",
   "metadata": {},
   "source": [
    "## Problem 3.1\n",
    "\n",
    "**Consider a variable $x$ which is Bernoulli distributed with parameter $\\lambda$.  Show that the mean $\\mathrm{E}[x]$ is $\\lambda$ and the variance $\\mathrm{E}[(x - \\mathrm{E}[x])^2]$ is $\\lambda(1 - \\lambda)$.**"
   ]
  },
  {
   "cell_type": "markdown",
   "metadata": {},
   "source": [
    "\\begin{equation}\n",
    "\\begin{split}\n",
    "  Pr(x) &= \\mathrm{Bern}_x(\\lambda) \\\\\n",
    "        &= \\lambda^x(1 - \\lambda)^{1-x} \\\\\n",
    "\\end{split}\n",
    "\\end{equation}\n",
    "\n",
    "\\begin{equation}\n",
    "\\begin{split}\n",
    "  \\mathrm{E}[x] &= \\displaystyle\\sum_{x = 0,1}x\\lambda^x(1 - \\lambda)^{1-x} \\\\\n",
    "                &= 1\\cdot\\lambda + 0\\cdot(1 - \\lambda) \\\\\n",
    "                &= \\lambda\n",
    "\\end{split}\n",
    "\\end{equation}\n",
    "\n",
    "Since\n",
    "\\begin{equation}\n",
    "\\begin{split}\n",
    "  \\mathrm{E}[x^2] &= \\displaystyle\\sum_{x = 0,1}x^2\\lambda^x(1 - \\lambda)^{1-x} \\\\\n",
    "                  &= 1^2\\cdot\\lambda + 0^2\\cdot(1 - \\lambda) \\\\\n",
    "                  &= \\lambda\n",
    "\\end{split}\n",
    "\\end{equation}\n",
    "\n",
    "then\n",
    "\n",
    "\\begin{equation}\n",
    "\\begin{split}\n",
    "  \\mathrm{E}[(x - \\mathrm{E}[x]] &= \\mathrm{E}[x^2] - \\mathrm{E}[x]^2 \\\\\n",
    "       &= \\lambda - \\lambda^2 \\\\\n",
    "       &= \\lambda(1 - \\lambda)\n",
    "\\end{split}\n",
    "\\end{equation}"
   ]
  },
  {
   "cell_type": "markdown",
   "metadata": {
    "collapsed": true
   },
   "source": [
    "## Problem 3.2\n",
    "\n",
    "**Calculate an expression for the mode (position of the peak) of the beta distribution with $\\alpha, \\beta > 1$ in terms of the parameters $\\alpha$ and $\\beta$.**"
   ]
  },
  {
   "cell_type": "markdown",
   "metadata": {},
   "source": [
    "The Beta distribution is written as:\n",
    "\n",
    "\\begin{equation}\n",
    "  Pr(\\lambda) = \\frac{\\Gamma(\\alpha + \\beta)}{\\Gamma(\\alpha) \\Gamma(\\beta)}\\lambda^{\\alpha-1}(1 - \\lambda)^{\\beta-1}\n",
    "\\end{equation}\n",
    "\n",
    "Then, the derivative of this distribution about $\\lambda$ is:\n",
    "\n",
    "\\begin{equation}\n",
    "\\begin{split}\n",
    "  \\frac{\\partial}{\\partial\\lambda}\\Pr(\\lambda) &= \\frac{\\Gamma(\\alpha + \\beta)}{\\Gamma(\\alpha) \\Gamma(\\beta)}\\bigl\\{(\\alpha-1)\\lambda^{\\alpha-2}(1 - \\lambda)^{\\beta-1} - (\\beta-1)\\lambda^{\\alpha-1}(1 - \\lambda)^{\\beta-2}) \\bigr\\} \\\\\n",
    "    &= \\frac{\\Gamma(\\alpha + \\beta)}{\\Gamma(\\alpha) \\Gamma(\\beta)}\\lambda^{\\alpha-1}(1 - \\lambda)^{\\beta-1}\\biggl(\\frac{\\alpha-1}{\\lambda} - \\frac{\\beta-1}{1-\\lambda}\\biggr) \\\\\n",
    "    &= \\Gamma(\\lambda)\\biggl(\\frac{\\alpha-1}{\\lambda} - \\frac{\\beta-1}{1-\\lambda}\\biggr)\n",
    "\\end{split}\n",
    "\\end{equation}\n",
    "\n",
    "Hense, the peak of this distribution is:\n",
    "\n",
    "\\begin{equation}\n",
    "  \\frac{\\partial}{\\partial \\lambda}\\Pr(\\lambda) = 0 \\implies \\frac{\\alpha-1}{\\lambda} - \\frac{\\beta-1}{1-\\lambda} = 0 \\\\\n",
    "  \\therefore \\lambda = \\frac{\\alpha - 1}{\\alpha + \\beta - 2}\n",
    "\\end{equation}"
   ]
  },
  {
   "cell_type": "markdown",
   "metadata": {
    "collapsed": true
   },
   "source": [
    "## Problem 3.3\n",
    "\n",
    "**The mean and variance of the beta distribution are given by the expressions$$\n",
    "\\begin{split}\n",
    "  E[\\lambda] = \\mu &= \\frac{\\alpha}{\\alpha + \\beta} \\\\\n",
    "  E[(\\lambda - \\mu)^2] = \\sigma^2 &= \\frac{\\alpha\\beta}{(\\alpha + \\beta)^2(\\alpha + \\beta + 1)}\n",
    "\\end{split}\n",
    "$$**\n",
    "\n",
    "**We may wish to choose the parameters $\\alpha$ and $\\beta$ so that the distribution has a particular mean $\\mu$ and variance $\\sigma^2$.  Derive suitable expressions for $\\alpha$ and $\\beta$ in terms of $\\mu$ and $\\sigma^2$.**"
   ]
  },
  {
   "cell_type": "markdown",
   "metadata": {
    "collapsed": true
   },
   "source": [
    "\\begin{align}\n",
    "  \\alpha &= \\mu\\biggl\\{\\frac{\\mu(1-\\mu)}{\\sigma^2} - 1\\biggr\\} \\\\\n",
    "  \\beta  &= (1 - \\mu)\\biggl\\{\\frac{\\mu(1-\\mu)}{\\sigma^2} - 1\\biggr\\}\n",
    "\\end{align}"
   ]
  },
  {
   "cell_type": "markdown",
   "metadata": {
    "collapsed": true
   },
   "source": [
    "## Problem 3.4\n",
    "\n",
    "**All of the distributions in this chapter are members of the _exponential family_ and can be written in the form$$\n",
    "  Pr(x|\\mathbf{\\theta}) = a[\\mathbf{x}]\\exp[\\mathbf{b}[\\mathbf{\\theta}]^T\\mathbf{c}[\\mathbf{x}]-d[\\mathbf{\\theta}]],\n",
    "$$ where $a[\\mathbf{x}]$ and $\\mathbf{c}[\\mathbf{x}]$ are functions of the data and $\\mathbf{b}[\\mathbf{\\theta}]$ and $d[\\mathbf{\\theta}]$ are functions of the parameters.  Find the functions $a[\\mathbf{x}]$, $\\mathbf{b}[\\mathbf{\\theta}]$, $\\mathbf{c}[\\mathbf{x}]$ and $d[\\mathbf{\\theta}]$ that allow the Beta distribution to be represented in the generalized form of the exponential family.**"
   ]
  },
  {
   "cell_type": "markdown",
   "metadata": {},
   "source": [
    "Define:\n",
    "\n",
    "\\begin{align}\n",
    "  a[\\mathbf{x}] &= 1 \\\\\n",
    "  \\mathbf{b}[\\mathbf{\\theta}] &= (\\alpha-1, \\beta-1)^T \\\\\n",
    "  \\mathbf{c}[\\mathbf{x}] &= (\\ln x, \\ln(1 - x))^T \\\\\n",
    "  d[\\mathbf{\\theta}] &= \\ln\\Gamma(\\alpha + \\beta) - \\ln\\Gamma(\\alpha) - \\ln\\Gamma(\\beta) \\\\\n",
    "\\end{align}\n",
    "\n",
    "Then the Beta distribution is written as:\n",
    "\n",
    "\\begin{equation}\n",
    "\\begin{split}\n",
    "  Pr(x) &= \\frac{\\Gamma(\\alpha + \\beta)}{\\Gamma(\\alpha)\\Gamma(\\beta)}x^{\\alpha-1}(1-x)^{\\beta-1}  \\\\\n",
    "              &= \\exp[\\ln[\\Gamma(\\alpha + \\beta)] - \\ln[\\Gamma(\\alpha)] - \\ln[\\Gamma(\\beta)] + (\\alpha-1)\\ln[x] + (\\beta-1)\\ln[1-x]] \\\\\n",
    "              &= a[\\mathbf{x}]\\exp[\\mathbf{b}[\\mathbf{\\theta}]^T\\mathbf{c}[\\mathbf{x}] - d[\\mathbf{\\theta}]]\n",
    "\\end{split}\n",
    "\\end{equation}"
   ]
  },
  {
   "cell_type": "markdown",
   "metadata": {
    "collapsed": true
   },
   "source": [
    "## Problem 3.5\n",
    "\n",
    "**Use integration by parts to prove that if $$\n",
    "  \\Gamma[z] = \\int_0^{\\infty}t^{z-1}e^{-t}dt,\n",
    "$$ then $$\n",
    "  \\Gamma[z + 1] = z\\Gamma[z].\n",
    "$$**"
   ]
  },
  {
   "cell_type": "markdown",
   "metadata": {},
   "source": [
    "\\begin{equation}\n",
    "\\begin{split}\n",
    "  \\Gamma[z + 1] &= \\int_0^{\\infty}t^{z}e^{-t}dt \\\\\n",
    "                &= \\int_0^{\\infty}t^{z}(-e^{-t})'dt \\\\\n",
    "                &= -t^{z}e^{-1}\\big\\vert_{t=0}^{t=\\infty} + \\int_0^{\\infty}\\frac{\\partial}{\\partial t}(t^{z})e^{-t}dt \\\\\n",
    "                &= z\\int_0^{\\infty}t^{z-1}e^{-t}dt \\\\\n",
    "                &= z\\Gamma[z]\n",
    "\\end{split}\n",
    "\\end{equation}"
   ]
  },
  {
   "cell_type": "markdown",
   "metadata": {
    "collapsed": true
   },
   "source": [
    "## Problem 3.6\n",
    "\n",
    "**Consider a restricted family of univariate normal distributions where the variance is always 1, so that $$\n",
    "    Pr(x|u) = \\frac{1}{\\sqrt{2\\pi}}\\exp\\bigl[-0.5(x - \\mu)^2\\bigr].\n",
    "$$**\n",
    "\n",
    "**Show that a normal distribution over the parameter $\\mu$ $$\n",
    "    Pr(\\mu) = \\text{Norm}_{\\mu}[\\mu_p, \\sigma_p^2]\n",
    "$$ has a conjugate relationship to the restricted normal distribution.**"
   ]
  },
  {
   "cell_type": "markdown",
   "metadata": {},
   "source": [
    "Since\n",
    "\n",
    "\\begin{equation}\n",
    "\\begin{split}\n",
    "  Pr(\\mu) &= \\text{Norm}_{\\mu}[\\mu_p, \\sigma_p^2] \\\\\n",
    "          &= \\frac{1}{\\sqrt{2\\pi\\sigma_p^2}}\\exp\\bigl[-0.5(\\mu - \\mu_p)^2/\\sigma_p^2\\bigr],\n",
    "\\end{split}\n",
    "\\end{equation}\n",
    "\n",
    "then\n",
    "\n",
    "\\begin{equation}\n",
    "\\begin{split}\n",
    "  Pr(x|\\mu)Pr(\\mu) &= \\text{Norm}_{\\mu}[\\mu_p, \\sigma_p^2] \\\\\n",
    "          &= \\frac{1}{\\sqrt{2\\pi}\\sqrt{2\\pi\\sigma_p^2}}\\exp\\bigl[-0.5(x - \\mu)^2 - 0.5(\\mu - \\mu_p)^2/\\sigma_p^2\\bigr] \\\\\n",
    "          &= \\frac{1}{\\sqrt{2\\pi}\\sqrt{2\\pi\\sigma_p^2}}\\exp\\bigl[-0.5\\bigl\\{(\\sigma_p^2 + 1)\\mu^2 - 2(x\\sigma_p^2 + \\mu_p)\\mu + x^2\\sigma_p^2 + \\mu_p^2\\bigr\\}/\\sigma_p^2\\bigr] \\\\\n",
    "          &= \\frac{1}{\\sqrt{2\\pi}\\sqrt{2\\pi\\sigma_p^2}}\\exp\\biggl[-0.5\\biggl\\{\\frac{\\mu^2 - 2(x\\sigma_p^2 + \\mu_p)\\mu\\big/(\\sigma_p^2 + 1)}{\\sigma_p^2/(\\sigma_p^2 + 1)} + \\frac{x^2\\sigma_p^2 + \\mu_p^2}{\\sigma_p^2}\\biggr\\}\\biggr] \\\\\n",
    "          &= \\frac{1}{\\sqrt{2\\pi}\\sqrt{2\\pi\\sigma_p^2}}\\exp\\biggl[-0.5\\biggl\\{\\frac{\\big(\\mu - (x\\sigma_p^2 + \\mu_p)\\big/(\\sigma_p^2 + 1)\\big)^2}{\\sigma_p^2/(\\sigma_p^2 + 1)} - \\frac{\\sigma_p^2 + 1}{\\sigma_p^2}\\biggl(\\frac{x\\sigma_p^2 + \\mu_p}{\\sigma_p^2 + 1}\\biggr)^2+ \\frac{x^2\\sigma_p^2 + \\mu_p^2}{\\sigma_p^2}\\biggr\\}\\biggr] \\\\\n",
    "          &= \\frac{1}{\\sqrt{2\\pi}\\sqrt{2\\pi\\sigma_p^2}}\\exp\\biggl[-0.5\\biggl\\{\\frac{\\big(\\mu - (x\\sigma_p^2 + \\mu_p)\\big/(\\sigma_p^2 + 1)\\big)^2}{\\sigma_p^2/(\\sigma_p^2 + 1)} + \\frac{x^2 - 2x\\mu_p + \\mu_p^2}{\\sigma_p^2 + 1}\\biggr\\}\\biggr] \\\\\n",
    "          &= \\frac{1}{\\sqrt{2\\pi}\\sqrt{2\\pi\\sigma_p^2}}\\exp\\biggl[-0.5\\biggl\\{\\frac{\\big(\\mu - (x\\sigma_p^2 + \\mu_p)\\big/(\\sigma_p^2 + 1)\\big)^2}{\\sigma_p^2/(\\sigma_p^2 + 1)} + \\frac{(x - \\mu_p)^2}{\\sigma_p^2 + 1}\\biggr\\}\\biggr] \\\\\n",
    "\\end{split}\n",
    "\\end{equation}\n",
    "\n",
    "Defining\n",
    "\n",
    "\\begin{align}\n",
    "  \\tilde{\\mu} &= \\frac{x\\sigma_p^2 + \\mu_p}{\\sigma_p^2 + 1} \\\\\n",
    "  \\tilde{\\sigma}^2 &= \\frac{\\sigma_p^2}{\\sigma_p^2 + 1},\n",
    "\\end{align}\n",
    "\n",
    "then the multiplication gets\n",
    "\n",
    "\\begin{equation}\n",
    "\\begin{split}\n",
    "  Pr(x|\\mu)Pr(\\mu) &= \\frac{1}{\\sqrt{2\\pi(\\sigma_p^2 + 1)}}\\exp\\biggl[-0.5\\frac{(x - \\mu_p^2)^2}{\\sigma_p^2 + 1}\\biggr] \\cdot \\frac{1}{\\sqrt{2\\pi\\tilde{\\sigma}^2}}\\exp\\biggl[-0.5\\frac{(\\mu - \\tilde{\\mu})^2}{\\tilde{\\sigma}^2}\\biggr] \\\\\n",
    "                   &= \\kappa(x, \\mu_p, \\sigma_p^2)\\text{Norm}_\\mu[\\tilde{\\mu}, \\tilde{\\sigma}^2]\n",
    "\\end{split}\n",
    "\\end{equation}\n",
    "\n",
    "Hense, a normal distirbution over the parameter $\\mu$ is conjugate to the restricted normal distribution."
   ]
  },
  {
   "cell_type": "markdown",
   "metadata": {},
   "source": [
    "## Problem 3.7\n",
    "\n",
    "**For the univariate normal distribution, find the functions $a[\\mathbf{x}]$, $\\mathbf{b}[\\mathbf{\\theta}]$, $\\mathbf{c}[\\mathbf{x}]$ and $d[\\mathbf{\\theta}]$ that allow it to be represented in the generalized form of the exponetential family.**"
   ]
  },
  {
   "cell_type": "markdown",
   "metadata": {
    "collapsed": true
   },
   "source": [
    "Define:\n",
    "\n",
    "\\begin{align}\n",
    "  a[\\mathbf{x}] &= 1 \\\\\n",
    "  \\mathbf{b}[\\mathbf{\\theta}] &= \\left(-\\frac{1}{2\\sigma^2}, \\frac{1}{\\sigma^2}\\right)^T \\\\\n",
    "  \\mathbf{c}[\\mathbf{x}] &= \\left(x^2, x \\right)^T \\\\\n",
    "  d[\\mathbf{\\theta}] &= \\frac{\\mu^2}{2\\sigma^2} + \\frac{1}{2}\\ln(2\\pi\\sigma^2) \\\\\n",
    "\\end{align}\n",
    "\n",
    "Then the univariate normal distribution is written as:\n",
    "\n",
    "\\begin{equation}\n",
    "\\begin{split}\n",
    "  Pr(x) &= \\text{Norm}_x[\\mu, \\sigma^2] \\\\\n",
    "        &= \\frac{1}{\\sqrt{2\\pi\\sigma^2}}\\exp\\biggl[-\\frac{(x - \\mu)^2}{2\\sigma^2}\\biggr] \\\\\n",
    "        &= \\exp\\biggl[\\ln\\frac{1}{\\sqrt{2\\pi\\sigma^2}}\\biggr]\\exp\\biggl[-\\frac{(x - \\mu)^2}{2\\sigma^2}\\biggr] \\\\\n",
    "        &= \\exp\\biggl[-\\frac{x^2}{2\\sigma^2} + \\frac{x}{\\sigma^2} - \\left(\\frac{\\mu^2}{2\\sigma^2} + \\frac{1}{2}\\ln(2\\pi\\sigma^2)\\right)\\biggr] \\\\\n",
    "        &= a[\\mathbf{x}]\\exp[\\mathbf{b}[\\mathbf{\\theta}]^T\\mathbf{c}[\\mathbf{x}]-d[\\mathbf{\\theta}]].\n",
    "\\end{split}\n",
    "\\end{equation}"
   ]
  },
  {
   "cell_type": "markdown",
   "metadata": {
    "collapsed": true
   },
   "source": [
    "## Problem 3.8\n",
    "\n",
    "Calculate an expression for the mode (position of the peak in $\\mu$, $\\sigma^2$ space) of the normal scaled inverse gamma distribution in terms of the parameters $\\alpha, \\beta, \\gamma, \\sigma$."
   ]
  },
  {
   "cell_type": "markdown",
   "metadata": {
    "collapsed": true
   },
   "source": [
    "The normal-scaled inverse gamma distribution is written as:\n",
    "\n",
    "\\begin{equation}\n",
    "  Pr(\\mu, \\sigma^2) = \\frac{\\sqrt{\\gamma}}{\\sigma\\sqrt{2\\pi}}\\frac{\\beta^{\\alpha}}{\\Gamma[\\alpha]}\\left(\\frac{1}{\\sigma^2}\\right)^{\\alpha+1}\\exp\\left[-\\frac{2\\beta + \\gamma(\\delta - \\mu)^2}{2\\sigma^2}\\right],\n",
    "\\end{equation}"
   ]
  },
  {
   "cell_type": "markdown",
   "metadata": {},
   "source": [
    "The partial derivatives in terms of $\\mu$ is written as:\n",
    "\n",
    "\\begin{equation}\n",
    "  \\frac{d}{d\\mu}Pr(\\mu, \\sigma^2) = \\frac{\\sqrt{\\gamma}}{\\sigma\\sqrt{2\\pi}}\\frac{\\beta^{\\alpha}}{\\Gamma[\\alpha]}\\left(\\frac{1}{\\sigma^2}\\right)^{\\alpha+1}\\exp\\left[-\\frac{2\\beta + \\gamma(\\delta - \\mu)^2}{2\\sigma^2}\\right] \\cdot \\frac{\\gamma(\\delta - \\mu)}{\\sigma^2}\n",
    "\\end{equation}\n",
    "\n",
    "This gives us the insight of the mode of $\\mu$:\n",
    "\n",
    "\\begin{equation}\n",
    "  \\frac{d}{d\\mu}Pr(\\mu, \\sigma^2) = 0 \\implies \\frac{\\gamma(\\delta - \\mu)}{\\sigma^2} = 0 \\\\\n",
    "\\end{equation}\n",
    "\\begin{equation}\n",
    "  \\therefore \\mu = \\delta\n",
    "\\end{equation}"
   ]
  },
  {
   "cell_type": "markdown",
   "metadata": {},
   "source": [
    "Next, the partial derivatives in terms of $\\sigma^2$ is written as:\n",
    "\n",
    "\\begin{equation}\n",
    "\\begin{split}\n",
    "  \\frac{d}{d\\sigma^2}Pr(\\mu, \\sigma^2) &= \\frac{d}{d\\sigma}Pr(\\mu, \\sigma^2)\\frac{d\\sigma}{d\\sigma^2} \\\\\n",
    "       &= \\frac{\\sqrt{\\gamma}}{\\sqrt{2\\pi}}\\frac{\\beta^{\\alpha}}{\\Gamma[\\alpha]}\\exp\\left[-\\frac{2\\beta + \\gamma(\\delta - \\mu)^2}{2\\sigma^2}\\right]\n",
    "          \\left[\\left(\\frac{1}{\\sigma}\\right)'\\left(\\frac{1}{\\sigma^2}\\right)^{\\alpha+1} + \\frac{1}{\\sigma}\\left\\{\\left(\\frac{1}{\\sigma^2}\\right)^{\\alpha+1}\\right\\}' + \\frac{1}{\\sigma}\\left(\\frac{1}{\\sigma^2}\\right)^{\\alpha+1}\\left\\{-\\frac{2\\beta + \\gamma(\\delta - \\mu)^2}{2\\sigma^2}\\right\\}'\\right]\\frac{1}{2\\sigma} \\\\\n",
    "       &= \\frac{\\sqrt{\\gamma}}{\\sqrt{2\\pi}}\\frac{\\beta^{\\alpha}}{\\Gamma[\\alpha]}\\exp\\left[-\\frac{2\\beta + \\gamma(\\delta - \\mu)^2}{2\\sigma^2}\\right]\n",
    "          \\left[-\\frac{1}{\\sigma^2}\\left(\\frac{1}{\\sigma^2}\\right)^{\\alpha+1} + \\frac{1}{\\sigma}(\\alpha+1)\\left(\\frac{1}{\\sigma^2}\\right)^{\\alpha}\\left(-\\frac{2}{\\sigma^3}\\right) + \\frac{1}{\\sigma}\\left(\\frac{1}{\\sigma^2}\\right)^{\\alpha+1}\\frac{2\\beta + \\gamma(\\delta - \\mu)^2}{\\sigma^3}\\right]\\frac{1}{2\\sigma} \\\\\n",
    "       &= \\frac{\\sqrt{\\gamma}}{\\sqrt{2\\pi}}\\frac{\\beta^{\\alpha}}{\\Gamma[\\alpha]}\\exp\\left[-\\frac{2\\beta + \\gamma(\\delta - \\mu)^2}{2\\sigma^2}\\right]\n",
    "          \\left[-(2\\alpha + 3) + \\frac{2\\beta + \\gamma(\\delta - \\mu)^2}{\\sigma^2}\\right]\\left(\\frac{1}{\\sigma^2}\\right)^{\\alpha+2}\\frac{1}{2\\sigma} \\\\\n",
    "\\end{split}\n",
    "\\end{equation}\n",
    "\n",
    "The condition of the mode of $\\sigma^2$ is:\n",
    "\n",
    "\\begin{equation}\n",
    "  \\frac{d}{d\\mu}Pr(\\mu, \\sigma^2)\\bigg\\vert_{\\mu=\\delta} = 0 \\implies -(2\\alpha + 3) + \\frac{2\\beta}{\\sigma^2} = 0 \\\\\n",
    "\\end{equation}\n",
    "\\begin{equation}\n",
    "  \\therefore \\sigma^2 = \\frac{2\\beta}{2\\alpha + 3}\n",
    "\\end{equation}"
   ]
  },
  {
   "cell_type": "markdown",
   "metadata": {
    "collapsed": true
   },
   "source": []
  }
 ],
 "metadata": {
  "_draft": {
   "nbviewer_url": "https://gist.github.com/2d15fe00f6d49edd140b38d825455687"
  },
  "gist": {
   "data": {
    "description": "CVmodels/Ch.03 Common probability distributions.ipynb",
    "public": true
   },
   "id": "2d15fe00f6d49edd140b38d825455687"
  },
  "hide_input": false,
  "kernelspec": {
   "display_name": "Python 3",
   "language": "python",
   "name": "python3"
  },
  "language_info": {
   "codemirror_mode": {
    "name": "ipython",
    "version": 3
   },
   "file_extension": ".py",
   "mimetype": "text/x-python",
   "name": "python",
   "nbconvert_exporter": "python",
   "pygments_lexer": "ipython3",
   "version": "3.6.2"
  },
  "toc": {
   "colors": {
    "hover_highlight": "#DAA520",
    "navigate_num": "#000000",
    "navigate_text": "#333333",
    "running_highlight": "#FF0000",
    "selected_highlight": "#FFD700",
    "sidebar_border": "#EEEEEE",
    "wrapper_background": "#FFFFFF"
   },
   "moveMenuLeft": true,
   "nav_menu": {
    "height": "30px",
    "width": "252px"
   },
   "navigate_menu": true,
   "number_sections": false,
   "sideBar": true,
   "threshold": 4,
   "toc_cell": false,
   "toc_section_display": "block",
   "toc_window_display": false,
   "widenNotebook": false
  }
 },
 "nbformat": 4,
 "nbformat_minor": 2
}
